LeanScratch/Computation/RegTree.lean
@@ -1,0 +1,33 @@
+import LeanScratch.Vec
+import LeanScratch.Fin2
+
+namespace Comp
+
+inductive RegTree
+  | lf (n : Nat)
+  | br (l r : RegTree)
+
+abbrev RegTree.toStore : RegTree → Type
+  | .lf n => Vec Nat n
+  | .br l r => l.toStore × r.toStore
+
+def Vec.zero {n} : Vec Nat n :=
+  match n with
+  | 0 => %[]
+  | _+1 => 0 %::zero
+
+def RegTree.toStore.zero {r : RegTree} : r.toStore :=
+  match r with
+  | .lf _ => Vec.zero
+  | .br _ _ => ⟨zero, zero⟩
+
+instance {r : RegTree} : Repr r.toStore where
+  reprPrec v _ := f v
+    where
+      f {r : RegTree} (v : r.toStore) : Std.Format := match r with
+      | .lf _ => repr v
+      | .br _ _ => .bracket "⟨" (f v.fst ++ ", " ++ f v.snd) "⟩"
+
+abbrev RegTree.toIdx : RegTree → Type
+  | .lf n => Fin2 n
+  | .br l r => l.toIdx ⊕ r.toIdx
