LeanScratch/Computation/Subprogram.lean
@@ -1,0 +1,10 @@
+import LeanScratch.Computation.RegMachine
+
+namespace Comp
+
+def transformReg
+    {r t : RegTree}
+    (f : r.toIdx → t.toIdx)
+    (inM : RegMachine r L)
+    : RegMachine t L := sorry
+
